Finish strong normalization proof of STLC+errors and soundness of CEK

src/Eval.v
@@ -1,11 +1,14 @@
 Require Import
   Lib
+  Ltac
   Ty
   Exp
+  Log
   Value
   Sub
   Sem
   Step
+  Multi
   Lang.
 
 From Equations Require Import Equations.
@@ -20,29 +23,37 @@ Import ListNotations.
 Context {A : Type}.
 Context `{L : HostLang A}.
 
-Inductive Kont : Ty → Ty → Type :=
-  | MT {a}   : Kont a a
-  | FN {a b} : (Value a → Σ b) → Kont a b
+Inductive Closed : Ty → Type :=
+  | Closure {Γ τ} : Exp Γ τ → ClEnv Γ → Closed τ
+  (* | Clapp {dom cod} : Closed (dom ⟶ cod) → Closed dom → Closed cod *)
 
-with Σ : Ty → Type :=
-  | MkΣ {Γ    : Env}
+with ClEnv : Env → Type :=
+  | NoCl : ClEnv []
+  | AddCl {Γ τ} : Value τ → ClEnv Γ → ClEnv (τ :: Γ)
+
+with Value : Ty → Type :=
+  | Val {Γ τ} (x : Exp Γ τ) : ValueP x → ClEnv Γ → Value τ.
+
+Derive Signature NoConfusion NoConfusionHom Subterm for ClEnv Closed Value.
+
+Equations get_val `(s : ClEnv Γ) `(v : Var Γ τ) : Value τ :=
+  get_val (AddCl x _)  ZV     := x;
+  get_val (AddCl _ xs) (SV v) := get_val xs v.
+
+Inductive EvalContext : Ty → Ty → Type :=
+  | MT {τ} : EvalContext τ τ
+  | AR {dom cod τ} : Closed dom → EvalContext cod τ → EvalContext (dom ⟶ cod) τ
+  | FN {dom cod τ} : Value (dom ⟶ cod) → EvalContext cod τ → EvalContext dom τ.
+
+Derive Signature NoConfusion NoConfusionHom Subterm for EvalContext.
+
+Inductive Σ : Ty → Type :=
+  | MkΣ {u    : Ty}
+        (exp  : Closed u)
         {τ    : Ty}
-        {r    : Ty}
-        (exp  : Exp Γ r)
-        (env  : ValEnv Γ)
-        (knt  : Kont r τ) : Σ τ.
+        (knt  : EvalContext u τ) : Σ τ.
 
-Derive Signature NoConfusion Subterm for Kont.
 Derive Signature NoConfusion NoConfusionHom Subterm for Σ.
-
-Equations with_closure `(a : Exp Γ dom) `(ρ : ValEnv Γ)
-          `(κ : Kont cod τ) `(f : Value (dom ⟶ cod)) : Σ τ :=
-  with_closure a ρ κ (ClosureExp (Lambda e)) :=
-    MkΣ a ρ (FN (λ v, MkΣ e (Val v Empty) κ));
-  (* with_closure a ρ κ (ClosureExp (Func f)) := *)
-  (*   MkΣ a ρ (FN (λ v, let '(existT _ x H) := valueToExp v in *)
-  (*                     MkΣ (CallHost f x H) Empty κ)) *)
-.
 
 (*
 Equations IfBody `(v : Value TyBool) {Γ τ} (t e : Exp Γ τ) : Exp Γ τ :=
@@ -72,55 +83,57 @@ Equations VIsNil `(v : Value (TyList r)) `(κ : Kont TyBool τ) : Σ τ :=
 
 Equations step {τ : Ty} (s : Σ τ) : Σ τ :=
   (* Constants *)
-  step (MkΣ (r:=TyHost _)   (HostedVal x) ρ (FN f)) := f (HostValue x);
-  step (MkΣ (r:=dom ⟶ cod) (HostedFun x) ρ (FN f)) := f (ClosureExp (Func x));
-  step (MkΣ (HostedExp x) ρ κ) := MkΣ (projT1 (Reduce x)) ρ κ;
+  (* step (MkΣ (r:=TyHost _)   (HostedVal x) ρ (FN f)) := f (HostValue x); *)
+  (* step (MkΣ (r:=dom ⟶ cod) (HostedFun x) ρ (FN f)) := f (ClosureExp (Func x)); *)
+  (* step (MkΣ (HostedExp x) ρ κ) := MkΣ (projT1 (Reduce x)) ρ κ; *)
 
-  step (MkΣ EUnit  _ (FN f)) := f VUnit;
-  step (MkΣ ETrue  _ (FN f)) := f VTrue;
-  step (MkΣ EFalse _ (FN f)) := f VFalse;
+  (* step (MkΣ EUnit  _ (FN f)) := f VUnit; *)
+  (* step (MkΣ ETrue  _ (FN f)) := f VTrue; *)
+  (* step (MkΣ EFalse _ (FN f)) := f VFalse; *)
 
-  step (MkΣ (If b th el) ρ κ) :=
-    MkΣ b ρ (FN (λ v, MkΣ (IfBody v th el) ρ κ));
+  (* step (MkΣ (If b th el) ρ κ) := *)
+  (*   MkΣ b ρ (FN (λ v, MkΣ (IfBody v th el) ρ κ)); *)
 
-  step (MkΣ (Pair x y) ρ (FN f)) :=
-    MkΣ x ρ (FN (λ v1, MkΣ y ρ (FN (λ v2, f (VPair v1 v2)))));
-  step (MkΣ (Fst p) ρ κ) :=
-    MkΣ p ρ (FN (λ p, MkΣ (projT1 (valueToExp (VFst p))) Empty κ));
-  step (MkΣ (Snd p) ρ κ) :=
-    MkΣ p ρ (FN (λ p, MkΣ (projT1 (valueToExp (VSnd p))) Empty κ));
+  (* step (MkΣ (Pair x y) ρ (FN f)) := *)
+  (*   MkΣ x ρ (FN (λ v1, MkΣ y ρ (FN (λ v2, f (VPair v1 v2))))); *)
+  (* step (MkΣ (Fst p) ρ κ) := *)
+  (*   MkΣ p ρ (FN (λ p, MkΣ (projT1 (valueToExp (VFst p))) Empty κ)); *)
+  (* step (MkΣ (Snd p) ρ κ) := *)
+  (*   MkΣ p ρ (FN (λ p, MkΣ (projT1 (valueToExp (VSnd p))) Empty κ)); *)
 
-  step (MkΣ Nil _ (FN f)) := f VNil;
-  step (MkΣ (Cons x xs) ρ (FN f)) :=
-    MkΣ x ρ (FN (λ v1, MkΣ xs ρ (FN (λ v2, f (VCons v1 v2)))));
-  step (MkΣ (Car d xs) ρ κ) :=
-    MkΣ xs ρ (FN (λ l, VCar l d ρ κ));
-  step (MkΣ (Cdr xs) ρ κ) :=
-    MkΣ xs ρ (FN (λ l, VCdr l ρ κ));
-  step (MkΣ (IsNil xs) ρ κ) :=
-    MkΣ xs ρ (FN (λ l, VIsNil l κ));
+  (* step (MkΣ Nil _ (FN f)) := f VNil; *)
+  (* step (MkΣ (Cons x xs) ρ (FN f)) := *)
+  (*   MkΣ x ρ (FN (λ v1, MkΣ xs ρ (FN (λ v2, f (VCons v1 v2))))); *)
+  (* step (MkΣ (Car d xs) ρ κ) := *)
+  (*   MkΣ xs ρ (FN (λ l, VCar l d ρ κ)); *)
+  (* step (MkΣ (Cdr xs) ρ κ) := *)
+  (*   MkΣ xs ρ (FN (λ l, VCdr l ρ κ)); *)
+  (* step (MkΣ (IsNil xs) ρ κ) := *)
+  (*   MkΣ xs ρ (FN (λ l, VIsNil l κ)); *)
 
-  (* A sequence just evaluates the second, for now *)
-  step (MkΣ (Seq e1 e2) ρ κ) := MkΣ e2 ρ κ;
+  (* (* A sequence just evaluates the second, for now *) *)
+  (* step (MkΣ (Seq e1 e2) ρ κ) := MkΣ e2 ρ κ; *)
 
   (* A variable might lookup a lambda, in which case continue evaluating down
      that vein; otherwise, if no continuation, this is as far as we can go. *)
-  step (MkΣ (VAR v) ρ κ) with get_value ρ v := {
-    | x with κ := {
-        | MT   => MkΣ (projT1 (valueToExp x)) Empty κ
-        | FN f => f x
-      }
+  step (MkΣ (Closure (VAR v) ρ) κ) with get_val ρ v := {
+    | Val (LAM e) _ ρ' := MkΣ (Closure (LAM e) ρ') κ
   };
 
   (* If a lambda is passed, call it with the continuation *)
-  step (MkΣ (LAM e) ρ (FN f)) := f (ClosureExp (Lambda (vsubst e ρ)));
+  step (MkΣ (Closure (LAM e) ρ) (AR a κ)) :=
+    MkΣ a (FN (Val (LAM e) (LambdaP _) ρ) κ);
+  step (MkΣ (Closure (LAM e) ρ) (FN (Val (LAM f) _ ρ') κ)) :=
+    MkΣ (Closure f (AddCl (Val (LAM e) (LambdaP _) ρ) ρ')) κ;
 
   (* Application evaluates the lambda and then the argument *)
-  step (MkΣ (APP e1 e2) ρ κ) := MkΣ e1 ρ (FN (with_closure e2 ρ κ));
+  step (MkΣ (Closure (APP f x) ρ) κ) :=
+    MkΣ (Closure f ρ) (AR (Closure x ρ) κ);
 
-  step (MkΣ e ρ MT) := MkΣ e ρ MT.
+  step (MkΣ (Closure (Error m) ρ) κ) := MkΣ (Closure (Error m) ρ) κ;
 
-(*
+  step (MkΣ c MT) := MkΣ c MT.
+
 Equations loop (gas : nat) {τ : Ty} (s : Σ τ) : Σ τ :=
   loop O s := s;
   loop (S gas') s := loop gas' (step s).
@@ -128,27 +141,32 @@ Equations loop (gas : nat) {τ : Ty} (s : Σ τ) : Σ τ :=
 (* Inject the expression into a [Σ] whose final continuation will receive the
    results of the evaluation. Therefore, the resulting [env] will be a
    singleton list containing that value. *)
-Definition inject {τ : Ty} (e : Exp [] τ) : Σ τ := MkΣ e Empty MT.
+Definition inject {τ : Ty} (e : Exp [] τ) : Σ τ := MkΣ (Closure e NoCl) MT.
 
 Definition run (gas : nat) {τ : Ty} (e : Exp [] τ) : Σ τ := loop gas (inject e).
 
-Ltac ceksimp :=
-  repeat (simp loop;
-          simp step;
-          simp IfBody;
-          simp VFst;
-          simp VSnd;
-          simpl).
+Definition Completes {τ} :=
+  ExpP (Γ:=[]) (τ:=τ) (λ _ e, ∃ e' gas, loop gas (inject e) = inject e').
 
-Ltac is_step := ceksimp; firstorder eauto.
-*)
+Definition completes_impl {τ} {e : Exp [] τ} :
+  Completes (τ:=τ) e → ∃ e' gas, loop gas (inject e) = inject e' := ExpP_P _.
 
-(*
-Theorem cek_sound τ (e e' : Exp [] τ) :
-  e --->* e' → ValueP e' →      (* evaluation halts at e' *)
-  ∃ gas, loop gas (inject e) = MkΣ e' Empty MT.
+Theorem all_exprs_complete τ (e e' : Exp [] τ) :
+  e --->* e' → Completes e.
 Proof.
-Abort.
-*)
+  intros.
+  unfold Completes.
+  induction τ.
+  now eapply IHτ2; eauto.
+Qed.
+
+Theorem cek_sound τ (e e' : Exp [] τ) :
+  e --->* e' → ∃ gas, loop gas (inject e) = inject e'.
+Proof.
+  intros.
+  apply all_exprs_complete in H.
+  induction τ.
+  exact (IHτ1 e e' H).
+Qed.
 
 End Eval.
